---
title: 779. K-th Symbol in Grammar
permalink: /docs/779
parent: misc
has_children: false
nav_order: 4
---
# 779. K-th Symbol in Grammar

[leetcode link](https://leetcode.com/problems/k-th-symbol-in-grammar/)

**difficulty(1-5)** 
4

**notes**

## Description

On the first row, we write a 0. Now in every subsequent row, we look at the previous row and replace each occurrence of 0 with 01, and each occurrence of 1 with 10.

Given row N and index K, return the K-th indexed symbol in row N. (The values of K are 1-indexed.) (1 indexed).

Examples:
Input: N = 1, K = 1
Output: 0

Input: N = 2, K = 1
Output: 0

Input: N = 2, K = 2
Output: 1

Input: N = 4, K = 5
Output: 1

Explanation:
row 1: 0
row 2: 01
row 3: 0110
row 4: 01101001
Note:

N will be an integer in the range [1, 30].
K will be an integer in the range [1, 2^(N-1)].

## Solution

Think of it as a full binary tree. 

If the node is 0, it generates 0 as left child and 1 as right child. 
If the node is 1, it generates 1 as left child and 0 as right child.

K is even, it's right child, odd then it's left child. We can use this information to go up to N-1 layer. 

Now we found the iteration :) 

more explanation: [link](https://leetcode.com/problems/k-th-symbol-in-grammar/discuss/113697/My-3-lines-C%2B%2B-recursive-solution)

```c++
class Solution {
public:
    int kthGrammar(int N, int K) {
        if (N == 1){
            return 0;
        }
        if (K%2 == 0){ // K is right child
            return (kthGrammar(N-1, K/2) == 0) ? 1 : 0;            
        }
        //else K is left child
        return (kthGrammar(N-1, (K+1)/2) == 0) ? 0 : 1;        
    }
};
``` 

<!-- 
Default label
{: .label }

Blue label
{: .label .label-blue }

Stable
{: .label .label-green }

New release
{: .label .label-purple }

Coming soon
{: .label .label-yellow }

Deprecated
{: .label .label-red } -->
